lexer/regexpScript.sml
@@ -76,6 +76,23 @@ Induct_on `rs` >>
 rw [fetch "-" "regexp_size_def"] >>
 full_simp_tac (srw_ss()++ARITH_ss) []);
 
+(* Check if a regexp matches nothing.  Neg r should match nothing iff r matches
+ * every possible string; however, that is not easy to determine, so we're
+ * conservative here and just say that Neg r might always match something *)
+val is_regexp_empty_def = tDefine "is_regexp_empty"`
+(is_regexp_empty (CharSet cs) = (cs = {})) ∧
+(is_regexp_empty (StringLit _) = F) ∧
+(is_regexp_empty (Cat r1 r2) = is_regexp_empty r1 ∨ is_regexp_empty r2) ∧
+(is_regexp_empty (Star _) = F) ∧
+(is_regexp_empty (Plus r) = is_regexp_empty r) ∧
+(is_regexp_empty (Or rs) = EVERY is_regexp_empty rs) ∧
+(is_regexp_empty (Neg r) = F)`
+(WF_REL_TAC `measure regexp_size` >>
+srw_tac [ARITH_ss] [] >>
+Induct_on `rs` >>
+rw [fetch "-" "regexp_size_def"] >>
+full_simp_tac (srw_ss()++ARITH_ss) []);
+
 val deriv_def = tDefine "deriv" `
 (deriv c (CharSet cs) =
   if c ∈ cs then
@@ -111,15 +128,20 @@ val deriv_matches_def = Define `
 (deriv_matches r "" = nullable r) ∧
 (deriv_matches r (c::s) = deriv_matches (deriv c r) s)`;
 
-val regexp_char_set_def = Define `
-regexp_char_set cs = CharSet cs`;
+val build_char_set_def = Define `
+build_char_set cs = CharSet cs`;
 
-val regexp_string_lit_def = Define `
-(regexp_string_lit "" = Star (CharSet {})) ∧
-(regexp_string_lit (c::s) = Cat (CharSet {c}) (regexp_string_lit s))`;
+val build_string_lit_def = Define `
+(build_string_lit "" = Star (CharSet {})) ∧
+(build_string_lit [c] = CharSet {c}) ∧
+(build_string_lit (c1::c2::s) = Cat (CharSet {c1}) (build_string_lit (c2::s)))`;
 
-val regexp_cat_def = Define `
-regexp_cat r1 r2 =
+val assoc_cat_def = Define `
+(assoc_cat (Cat r1 r2) r3 = Cat r1 (assoc_cat r2 r3)) ∧
+(assoc_cat r1 r2 = Cat r1 r2)`;
+
+val build_cat_def = Define `
+(build_cat r1 r2 =
   if (r1 = CharSet {}) ∨ (r2 = CharSet {}) then
     CharSet {}
   else if r1 = Star (CharSet {}) then
@@ -127,58 +149,142 @@ regexp_cat r1 r2 =
   else if r2 = Star (CharSet {}) then
     r1
   else
-    case r1 of
-      | Cat r3 r4 => regexp_cat r3 (Cat r4 r2)
-      | _ => Cat r1 r2`;
+    assoc_cat r1 r2)`;
 
-val regexp_neg_def = Define `
-(regexp_neg (Neg r) = r) ∧
-(regexp_neg r = (Neg r))`;
+val build_neg_def = Define `
+(build_neg (Neg r) = r) ∧
+(build_neg r = (Neg r))`;
 
-val regexp_star_def = Define `
-(regexp_star (Star r) = Star r) ∧
-(regexp_star r = Star r)`;
+val build_star_def = Define `
+(build_star (Star r) = Star r) ∧
+(build_star r = Star r)`;
 
-val regexp_plus_def = Define `
-regexp_plus r = regexp_cat r (regexp_star r)`;
+val build_plus_def = Define `
+build_plus r = build_cat r (build_star r)`;
 
 val flatten_or_def = Define `
 (flatten_or [] = []) ∧
 (flatten_or (Or rs::rs') = rs ++ flatten_or rs') ∧
 (flatten_or (r::rs) = r :: flatten_or rs)`;
 
-val regexp_or_def = Define `
-regexp_or rs = 
+val build_or_def = Define `
+build_or rs = 
   let rs = flatten_or rs in
     if MEM (Neg (CharSet {})) rs then
       Neg (CharSet {})
     else
       (* TODO: We should sort, remove duplicates, and merge CharSets *)
-      case rs of
+      case (FILTER (\r. r ≠ CharSet {}) rs) of
         | [] => CharSet {}
         | [r] => r
         | res => Or res`;
 
-val normalize_regexp_def = tDefine "normalize_regexp" `
-(normalize_regexp (CharSet cs) = 
-  regexp_char_set cs) ∧
-(normalize_regexp (StringLit s) = 
-  regexp_string_lit s) ∧
-(normalize_regexp (Cat r1 r2) = 
-  regexp_cat (normalize_regexp r1) (normalize_regexp r2)) ∧
-(normalize_regexp (Star r) =
-  regexp_star (normalize_regexp r)) ∧
-(normalize_regexp (Plus r) =
-  regexp_plus (normalize_regexp r)) ∧
-(normalize_regexp (Or rs) =
-  regexp_or (MAP normalize_regexp rs)) ∧
-(normalize_regexp (Neg r) =
-  regexp_neg (normalize_regexp r))`
+val regexp_smart_constructors_def = 
+  save_thm ("regexp_smart_constructors_def",
+            LIST_CONJ [build_or_def, build_plus_def, build_star_def,
+            build_cat_def, build_string_lit_def, build_char_set_def,
+            assoc_cat_def, build_neg_def]);
+
+val normalize_def = tDefine "normalize" `
+(normalize (CharSet cs) = 
+  build_char_set cs) ∧
+(normalize (StringLit s) = 
+  build_string_lit s) ∧
+(normalize (Cat r1 r2) = 
+  build_cat (normalize r1) (normalize r2)) ∧
+(normalize (Star r) =
+  build_star (normalize r)) ∧
+(normalize (Plus r) =
+  build_plus (normalize r)) ∧
+(normalize (Or rs) =
+  build_or (MAP normalize rs)) ∧
+(normalize (Neg r) =
+  build_neg (normalize r))`
 (WF_REL_TAC `measure regexp_size` >>
 srw_tac [ARITH_ss] [] >>
 Induct_on `rs` >>
 rw [regexp_size_def] >>
 full_simp_tac (srw_ss()++ARITH_ss) []);
+
+val normalize_ind =  (fetch "-" "normalize_ind")
+
+val is_normalized_def = tDefine "is_normalized" `
+(is_normalized (CharSet cs) = 
+  T) ∧
+(is_normalized (StringLit s) = 
+  F) ∧
+(is_normalized (Cat r1 r2) = 
+  (r1 ≠ CharSet {}) ∧
+  (r2 ≠ CharSet {}) ∧
+  (r1 ≠ Star (CharSet {})) ∧
+  (r2 ≠ Star (CharSet {})) ∧
+  (case r1 of 
+     | Cat _ _ => F
+     | _ => T) ∧
+  (is_normalized r1) ∧
+  (is_normalized r2)) ∧
+(is_normalized (Star r) =
+  is_normalized r ∧
+  (case r of
+     | Star _ => F
+     | _ => T)) ∧
+(is_normalized (Plus r) =
+  F) ∧
+(is_normalized (Or rs) =
+  LENGTH rs > 1 ∧
+  EVERY (\r. is_normalized r ∧
+             (case r of
+                 | Or _ => F
+                 | _ => T) ∧
+             (r ≠ Neg (CharSet {})) ∧
+             (r ≠ CharSet {}))
+        rs) ∧
+(is_normalized (Neg r) =
+  is_normalized r ∧
+  (case r of
+     | Neg _ => F
+     | _ => T))`
+(WF_REL_TAC `measure regexp_size` >>
+srw_tac [ARITH_ss] [] >>
+Induct_on `rs` >>
+rw [regexp_size_def] >>
+full_simp_tac (srw_ss()++ARITH_ss) []);
+
+
+val smart_deriv_def = tDefine "smart_deriv" `
+(smart_deriv c (CharSet cs) =
+  if c ∈ cs then
+    (build_string_lit "")
+  else
+    build_char_set {}) ∧
+(smart_deriv c (StringLit "") =
+  build_char_set {}) ∧
+(smart_deriv c (StringLit (c'::s)) =
+  if c = c' then
+    build_string_lit s
+  else
+    build_char_set {}) ∧
+(smart_deriv c (Cat r1 r2) =
+  let cat = build_cat (smart_deriv c r1) r2 in
+    if nullable r1 then
+      build_or [cat; (smart_deriv c r2)]
+    else
+      cat) ∧
+(smart_deriv c (Star r) =
+  build_cat (smart_deriv c r) (build_star r)) ∧
+(smart_deriv c (Plus r) = 
+  build_cat (smart_deriv c r) (build_star r)) ∧
+(smart_deriv c (Or rs) = build_or (MAP (smart_deriv c) rs)) ∧
+(smart_deriv c (Neg r) = build_neg (smart_deriv c r))`
+(WF_REL_TAC `measure (\(x,y). regexp_size y)` >>
+srw_tac [ARITH_ss] [] >>
+Induct_on `rs` >>
+rw [regexp_size_def] >>
+full_simp_tac (srw_ss()++ARITH_ss) []);
+
+val smart_deriv_matches_def = Define `
+(smart_deriv_matches r "" = nullable r) ∧
+(smart_deriv_matches r (c::s) = smart_deriv_matches (deriv c r) s)`;
 
 val nullable_thm = Q.store_thm ("nullable_thm",
 `!r. nullable r = regexp_matches r ""`,
@@ -356,5 +462,177 @@ metis_tac [APPEND_ASSOC] >|
      metis_tac [],
  fs [EXISTS_MEM] >>
      metis_tac []]);
+
+val regexp_empty_thm = Q.store_thm ("regexp_empty_thm",
+`!r l. is_regexp_empty r ⇒ ~regexp_matches r l`,
+recInduct (fetch "-" "is_regexp_empty_ind") >>
+rw [is_regexp_empty_def, regexp_matches_def, EVERY_EL] >>
+fs [is_regexp_empty_def, MEM_EL] >|
+[cases_on `ss` >>
+     rw [] >>
+     disj1_tac >>
+     qexists_tac `0` >>
+     decide_tac,
+ metis_tac []]);
+
+val assoc_cat_cat = Q.prove (
+`!r1 r2. ?r1' r2'. assoc_cat r1 r2 = Cat r1' r2'`,
+recInduct (fetch "-" "assoc_cat_ind") >>
+rw [assoc_cat_def]);
+
+val normalized_assoc_cat = Q.prove (
+`!r1 r2. 
+  (r1 ≠ CharSet {}) ∧
+  (r2 ≠ CharSet {}) ∧
+  (r1 ≠ Star (CharSet {})) ∧
+  (r2 ≠ Star (CharSet {})) ∧
+  is_normalized r1 ∧ 
+  is_normalized r2 
+  ⇒
+  is_normalized (assoc_cat r1 r2)`,
+recInduct (fetch "-" "assoc_cat_ind") >>
+rw [is_normalized_def, regexp_smart_constructors_def] >>
+cases_on `r1` >>
+fs [is_normalized_def] >>
+metis_tac [assoc_cat_cat, fetch "-" "regexp_distinct"]);
+
+val norm_string_lit = Q.prove (
+`!s. is_normalized (build_string_lit s)`,
+induct_on `s` >>
+     rw [] >> 
+     fs [is_normalized_def, regexp_smart_constructors_def] >>
+     cases_on `s` >>
+     fs [is_normalized_def, regexp_smart_constructors_def] >>
+     cases_on `t` >>
+     rw [] >> 
+     fs [is_normalized_def, regexp_smart_constructors_def]);
+
+val norm_char_set = Q.prove (
+`!cs. is_normalized (build_char_set cs)`,
+rw [is_normalized_def, regexp_smart_constructors_def]);
+
+val norm_cat = Q.prove (
+`!r1 r2. is_normalized r1 ∧ is_normalized r2 ⇒ is_normalized (build_cat r1 r2)`,
+rw [] >>
+cases_on `r1` >>
+fs [is_normalized_def, regexp_smart_constructors_def] >>
+rw [] >>
+fs [is_normalized_def, regexp_smart_constructors_def] >>
+rw [] >-
+metis_tac [assoc_cat_cat, fetch "-" "regexp_distinct"] >-
+metis_tac [assoc_cat_cat, fetch "-" "regexp_distinct"] >>
+match_mp_tac normalized_assoc_cat >>
+rw [is_normalized_def]);
+
+val norm_star = Q.prove (
+`!r. is_normalized r ⇒ is_normalized (build_star r)`,
+cases_on `r` >>
+rw [is_normalized_def, regexp_smart_constructors_def]);
+
+val norm_plus = Q.prove (
+`!r. is_normalized r ⇒ is_normalized (build_plus r)`,
+cases_on `r` >>
+rw [is_normalized_def, regexp_smart_constructors_def] >-
+metis_tac [assoc_cat_cat, fetch "-" "regexp_distinct"] >-
+metis_tac [assoc_cat_cat, fetch "-" "regexp_distinct"] >>
+match_mp_tac normalized_assoc_cat >>
+rw [is_normalized_def]);
+
+val norm_neg = Q.prove (
+`!r. is_normalized r ⇒ is_normalized (build_neg r)`,
+cases_on `r` >>
+rw [is_normalized_def, regexp_smart_constructors_def]);
+
+val flatten_or_thm = Q.prove (
+`!rs r. MEM r (flatten_or rs) ∧ EVERY is_normalized rs ⇒ ¬?rs'. r = Or rs'`,
+recInduct (fetch "-" "flatten_or_ind") >>
+rw [flatten_or_def] >>
+fs [is_normalized_def, EVERY_MEM] >>
+res_tac >>
+fs [] >>
+cases_on `r` >>
+fs []);
+
+val flatten_or_norm = Q.prove (
+`!rs r. EVERY is_normalized rs ⇒ EVERY is_normalized (flatten_or rs)`,
+recInduct (fetch "-" "flatten_or_ind") >>
+rw [flatten_or_def] >>
+fs [is_normalized_def, EVERY_MEM]);
+
+val norm_or = Q.prove (
+`!rs. EVERY is_normalized rs ⇒ is_normalized (build_or rs)`,
+rw [build_or_def, is_normalized_def] >>
+cases_on `MEM (Neg (CharSet ∅)) rs'` >>
+rw [is_normalized_def] >>
+`!r. MEM r rs' ⇒ ¬?rs'. r = Or rs'` by metis_tac [flatten_or_thm] >>
+cases_on `FILTER (λr. r ≠ CharSet ∅) rs'` >>
+fs [is_normalized_def] >>
+cases_on `t` >>
+fs [is_normalized_def, markerTheory.Abbrev_def, EVERY_MEM] >-
+metis_tac [flatten_or_norm, MEM, EVERY_MEM, MEM_FILTER] >>
+rw [] >|
+[decide_tac,
+ metis_tac [flatten_or_norm, MEM, EVERY_MEM, MEM_FILTER, FILTER],
+ `¬?rs'. h = Or rs'` by metis_tac [flatten_or_thm, MEM, EVERY_MEM, MEM_FILTER] >>
+     cases_on `h` >>
+     fs [],
+ metis_tac [MEM, EVERY_MEM, MEM_FILTER, FILTER],
+ `MEM h (FILTER (λr. r ≠ CharSet ∅) (flatten_or rs))` by metis_tac [MEM] >>
+     fs [MEM_FILTER],
+ metis_tac [flatten_or_norm, MEM, EVERY_MEM, MEM_FILTER, FILTER],
+ `¬?rs'. h' = Or rs'` by metis_tac [flatten_or_thm, MEM, EVERY_MEM, MEM_FILTER] >>
+     cases_on `h'` >>
+     fs [],
+ metis_tac [MEM, EVERY_MEM, MEM_FILTER, FILTER],
+ `MEM h' (FILTER (λr. r ≠ CharSet ∅) (flatten_or rs))` by metis_tac [MEM] >>
+     fs [MEM_FILTER],
+ metis_tac [flatten_or_norm, MEM, EVERY_MEM, MEM_FILTER, FILTER],
+ `¬?rs'. r = Or rs'` by metis_tac [flatten_or_thm, MEM, EVERY_MEM, MEM_FILTER] >>
+     cases_on `r` >>
+     fs [],
+ metis_tac [MEM, EVERY_MEM, MEM_FILTER, FILTER],
+ `MEM r (FILTER (λr. r ≠ CharSet ∅) (flatten_or rs))` by metis_tac [MEM] >>
+     fs [MEM_FILTER]]);
+
+val normalize_thm = Q.store_thm ("normalize_thm",
+`!r. is_normalized (normalize r)`,
+recInduct normalize_ind >>
+rw [normalize_def, norm_string_lit, norm_char_set, norm_cat, norm_neg,
+    norm_star, norm_plus] >>
+metis_tac [norm_or, EVERY_MEM, MEM_MAP]);
+
+val smart_deriv_normalized = Q.store_thm ("smart_deriv_normalized",
+`!c r. is_normalized r ⇒ is_normalized (smart_deriv c r)`,
+recInduct (fetch "-" "smart_deriv_ind") >>
+rw [is_normalized_def, smart_deriv_def, normalize_def, norm_string_lit,
+    norm_char_set, norm_cat, norm_neg, norm_star, norm_plus] >|
+[Q.UNABBREV_TAC `cat` >>
+     cases_on `nullable r1` >>
+     rw [is_normalized_def] >|
+     [match_mp_tac norm_or >>
+          rw [norm_cat],
+      rw [norm_cat]],
+ match_mp_tac norm_or >>
+     rw [EVERY_MAP] >> 
+     fs [EVERY_MEM]]);
+
+val norm_is_regexp_empty = Q.store_thm ("norm_is_regexp_empty",
+`!r. is_normalized r ⇒ (is_regexp_empty r = (r = CharSet {}))`,
+recInduct (fetch "-" "is_normalized_ind") >>
+rw [is_normalized_def, is_regexp_empty_def] >>
+fs [EXISTS_MEM, EVERY_MEM] >>
+rw [] >>
+cases_on `rs` >>
+rw [] >>
+fs [] >>
+metis_tac []);
+
+val regexp_matches_smart_deriv = Q.store_thm ("regexp_matches_smart_deriv",
+`!r s. regexp_matches r s = smart_deriv_matches r s`,
+cheat);
+
+val regexp_matches_normalize = Q.store_thm ("regexp_matches_normalize",
+`!r s. regexp_matches r s = regexp_matches (normalize r) s`,
+cheat);
 
 val _ = export_theory ();
